theories/L/Util/term_enum.v
@@ -1,0 +1,37 @@
+Require Import Undecidability.Synthetic.EnumerabilityFacts.
+Require Import Undecidability.L.L.
+Require Cantor.
+Require Import Lia.
+
+Fixpoint term_enum_rec (k n: nat) : term :=
+  match k with
+  | 0 => var 0
+  | S k => 
+    match Cantor.of_nat n with
+    | (0, n') => var n'
+    | (S (S n1), n2) => app (term_enum_rec k n1) (term_enum_rec k n2)
+    | (1, n') => lam (term_enum_rec k n')
+    end
+  end.
+
+Opaque Cantor.to_nat Cantor.of_nat.
+
+Definition term_enum (n : nat) := Some (term_enum_rec (S n) n).
+Lemma enumerator__T_term :
+  enumerator__T term_enum term.
+Proof.
+  intros t. unfold term_enum.
+  enough (exists n, forall m, n <= m -> term_enum_rec (S m) n = t) as [n Hn].
+  { exists n. f_equal. now apply Hn. }
+  induction t as [n|s [n1 IHs] t [n2 IHt]|s [n IH]].
+  - exists (Cantor.to_nat (0, n)). cbn.
+    now rewrite Cantor.cancel_of_to.
+  - exists (Cantor.to_nat (S (S n1), n2)). cbn.
+    assert (H' := Cantor.to_nat_non_decreasing (S (S n1)) n2).
+    intros [|m] ?. { lia. }
+    rewrite !Cantor.cancel_of_to, IHs, IHt; [easy | lia | lia].
+  - exists (Cantor.to_nat (1, n)). cbn.
+    assert (H' := Cantor.to_nat_non_decreasing 1 n).
+    intros [|m] ?. { lia. }
+    rewrite !Cantor.cancel_of_to, IH; [easy | lia ].
+Qed.
